VeriTile/Triton/DSL/Syntax.lean
@@ -146,6 +146,7 @@ syntax "tl.store(" tritonExpr ", " tritonExpr ("," tritonMemKwarg)* ")" : triton
 syntax "tl.atomic_add(" tritonExpr ", " tritonExpr ("," tritonMemKwarg)* ")" : tritonStmt
 syntax "tl.async_copy(" tritonExpr ", " tritonExpr ("," tritonMemKwarg)* ")" : tritonStmt
 syntax "tl.async_wait()" : tritonStmt
+syntax "tl.debug_barrier()" : tritonStmt
 syntax "tl.for " ident " in " "$(" term ")" " { " tritonStmt* " }" : tritonStmt
 syntax "tl.for " ident " in " num " { " tritonStmt* " }" : tritonStmt
 syntax "tl.static_range " ident " in " "$(" term ")" " { " tritonStmt* " }" : tritonStmt
